bedrock2/src/bedrock2/memory_mapped_ext_spec.v
@@ -1,0 +1,128 @@
+Require Import Coq.Strings.String. Local Open Scope string_scope.
+Require Import Coq.ZArith.ZArith.
+Require Import Coq.Lists.List. Import ListNotations. Local Open Scope list_scope.
+Require Import coqutil.Tactics.fwd coqutil.Tactics.autoforward.
+Require coqutil.Datatypes.String.
+Require Import coqutil.Map.Interface coqutil.Word.Interface coqutil.Word.Bitwidth.
+Require Import bedrock2.Semantics.
+Local Open Scope string_scope.
+
+#[local] Instance string_of_nbytes_inj: forall nbytes1 nbytes2,
+    autoforward (String.of_nat (nbytes1 * 8) = String.of_nat (nbytes2 * 8))
+                (nbytes1 = nbytes2).
+Proof.
+  intros * H.
+  eapply String.of_nat_inj in H.
+  eapply PeanoNat.Nat.mul_cancel_r. 2: eassumption.
+  discriminate.
+Qed.
+
+Class MemoryMappedExtCalls{width: Z}{BW: Bitwidth width}
+                          {word: word.word width} {mem: map.map word Byte.byte} := {
+  mmio_read_step:
+    nat -> (* how many bytes to read *)
+    trace -> (* trace of events that happened so far *)
+    word -> (* address to be read *)
+    (word -> mem -> Prop) -> (* postcondition on returned value and memory *)
+    Prop;
+  mmio_write_step:
+    nat -> (* how many bytes to write *)
+    trace -> (* trace of events that happened so far *)
+    word -> (* address to be written *)
+    word -> (* value to be written *)
+    mem -> (* memory whose ownership is passed to the external world *)
+    Prop;
+  (* same signatures for accessing shared memory, i.e. memory that has been passed
+     to the external world, but might still be accessible under some conditions,
+     and can change each time it is looked at *)
+  shared_mem_read_step:
+    nat -> (* how many bytes to read *)
+    trace -> (* trace of events that happened so far *)
+    word -> (* address to be read *)
+    (word -> mem -> Prop) -> (* postcondition on returned value and memory *)
+    Prop;
+  shared_mem_write_step:
+    nat -> (* how many bytes to write *)
+    trace -> (* trace of events that happened so far *)
+    word -> (* address to be written *)
+    word -> (* value to be written *)
+    mem -> (* memory whose ownership is passed to the external world *)
+    Prop;
+}.
+
+Section WithMem.
+  Context {width: Z} {BW: Bitwidth width}
+          {word: word.word width} {mem: map.map word Byte.byte}.
+  Context {word_ok: word.ok word}.
+
+  Inductive ext_spec{mmio_ext_calls: MemoryMappedExtCalls}: ExtSpec :=
+  | ext_spec_mmio_read: forall t addr n post,
+      mmio_read_step n t addr (fun v mRcv => post mRcv [v]) ->
+      ext_spec t map.empty ("MMIO_READ" ++ String.of_nat (n * 8)) [addr] post
+  | ext_spec_mmio_write: forall t addr n mGive v post,
+      mmio_write_step n t addr v mGive ->
+      post map.empty nil ->
+      ext_spec t mGive ("MMIO_WRITE" ++ String.of_nat (n * 8)) [addr; v] post
+  | ext_spec_shared_mem_read: forall t addr n post,
+      shared_mem_read_step n t addr (fun v mRcv => post mRcv [v]) ->
+      ext_spec t map.empty ("SHARED_MEM_READ" ++ String.of_nat (n * 8)) [addr] post
+  | ext_spec_shared_mem_write: forall t addr n mGive v post,
+      shared_mem_write_step n t addr v mGive ->
+      post map.empty nil ->
+      ext_spec t mGive ("SHARED_MEM_WRITE" ++ String.of_nat (n * 8)) [addr; v] post.
+
+  Class MemoryMappedExtCallsOk(mmio_ext_calls: MemoryMappedExtCalls): Prop := {
+    weaken_mmio_read_step: forall t addr n post1 post2,
+      mmio_read_step n t addr post1 ->
+      (forall v mRcv, post1 v mRcv -> post2 v mRcv) ->
+      mmio_read_step n t addr post2;
+    intersect_mmio_read_step: forall t addr n post1 post2,
+      mmio_read_step n t addr post1 ->
+      mmio_read_step n t addr post2 ->
+      mmio_read_step n t addr (fun v mRcv => post1 v mRcv /\ post2 v mRcv);
+    mmio_write_step_unique_mGive: forall m t n mKeep1 mKeep2 mGive1 mGive2 addr val,
+      map.split m mKeep1 mGive1 ->
+      map.split m mKeep2 mGive2 ->
+      mmio_write_step n t addr val mGive1 ->
+      mmio_write_step n t addr val mGive2 ->
+      mGive1 = mGive2;
+    weaken_shared_mem_read_step: forall t addr n post1 post2,
+      shared_mem_read_step n t addr post1 ->
+      (forall v mRcv, post1 v mRcv -> post2 v mRcv) ->
+      shared_mem_read_step n t addr post2;
+    intersect_shared_mem_read_step: forall t addr n post1 post2,
+      shared_mem_read_step n t addr post1 ->
+      shared_mem_read_step n t addr post2 ->
+      shared_mem_read_step n t addr (fun v mRcv => post1 v mRcv /\ post2 v mRcv);
+    shared_mem_write_step_unique_mGive: forall m t n mKeep1 mKeep2 mGive1 mGive2 addr val,
+      map.split m mKeep1 mGive1 ->
+      map.split m mKeep2 mGive2 ->
+      shared_mem_write_step n t addr val mGive1 ->
+      shared_mem_write_step n t addr val mGive2 ->
+      mGive1 = mGive2;
+  }.
+
+  Instance ext_spec_ok(mmio_ext_calls: MemoryMappedExtCalls)
+    {mmio_ext_calls_ok: MemoryMappedExtCallsOk mmio_ext_calls}: ext_spec.ok ext_spec.
+  Proof.
+    constructor.
+    - (* mGive unique *)
+      intros. inversion H1; subst; clear H1; inversion H2; subst; clear H2;
+        fwd; eauto using mmio_write_step_unique_mGive, shared_mem_write_step_unique_mGive.
+    - (* weaken *)
+      unfold Morphisms.Proper, Morphisms.respectful, Morphisms.pointwise_relation,
+        Basics.impl.
+      intros.
+      inversion H0; subst; clear H0;
+        constructor;
+        eauto using weaken_mmio_read_step, weaken_shared_mem_read_step.
+    - (* intersect *)
+      intros. inversion H; subst; clear H; inversion H0; subst; clear H0; fwd;
+        constructor;
+        eauto using intersect_mmio_read_step, intersect_shared_mem_read_step.
+  Qed.
+
+End WithMem.
+
+#[export] Existing Instance ext_spec.
+#[export] Existing Instance ext_spec_ok.
