compiler/src/compiler/memory_mapped_ext_calls_compiler.v
@@ -1,0 +1,168 @@
+Require Import Coq.ZArith.ZArith.
+Require Import coqutil.Z.Lia.
+Require Import coqutil.Tactics.fwd.
+Require Import compiler.util.Common.
+Require Import bedrock2.Semantics.
+Require Import riscv.Utility.Monads.
+Require Import riscv.Utility.FreeMonad.
+Require Import compiler.FlatImp.
+Require Import riscv.Spec.Decode.
+Require Import coqutil.sanity.
+Require Import riscv.Utility.MkMachineWidth.
+Require Import riscv.Spec.PseudoInstructions.
+Require Import riscv.Utility.InstructionCoercions.
+Require Import riscv.Spec.Machine.
+Require Import compiler.FlatToRiscvDef.
+Require Import compiler.FlatToRiscvCommon.
+Require Import compiler.FlatToRiscvFunctions.
+Require Import riscv.Platform.RiscvMachine.
+Require Import riscv.Spec.Primitives.
+Require Import riscv.Spec.MetricPrimitives.
+Require Import compiler.MetricsToRiscv.
+Require Import riscv.Utility.runsToNonDet.
+Require Import compiler.GoFlatToRiscv.
+Require Import compiler.SeparationLogic.
+Require Import coqutil.Datatypes.Option.
+Require Import compiler.RiscvWordProperties.
+Require Import coqutil.Datatypes.ListSet.
+
+(* Goal of this file: compile from this (bedrock2 ext calls): *)
+Require Import bedrock2.memory_mapped_ext_spec.
+(* to this (risc-v "ext calls" implemented by load and store instructions): *)
+Require Import compiler.memory_mapped_ext_calls_riscv.
+
+Import ListNotations.
+
+Local Open Scope bool_scope.
+Local Open Scope string_scope.
+
+Definition compile_load(action: string): Z -> Z -> Z -> Instruction :=
+  if (action =? "MMIO_READ64") || (action =? "SHARED_MEM_READ64") then Ld else
+  if (action =? "MMIO_READ32") || (action =? "SHARED_MEM_READ32") then Lw else
+  if (action =? "MMIO_READ16") || (action =? "SHARED_MEM_READ16") then Lh else Lb.
+
+Definition compile_store(action: string): Z -> Z -> Z -> Instruction :=
+  if (action =? "MMIO_WRITE64") || (action =? "SHARED_MEM_WRITE64") then Sd else
+  if (action =? "MMIO_WRITE32") || (action =? "SHARED_MEM_WRITE32") then Sw else
+  if (action =? "MMIO_WRITE16") || (action =? "SHARED_MEM_WRITE16") then Sh else Sb.
+
+Definition compile_interact(results: list Z)(a: string)(args: list Z): list Instruction :=
+  match results, args with
+  | [res], [addr] => [compile_load a res addr 0]
+  | [], [addr; val] => [compile_store a addr val 0]
+  | _, _ => [] (* invalid, excluded by ext_spec *)
+  end.
+
+Local Arguments Z.mul: simpl never.
+Local Arguments Z.add: simpl never.
+Local Arguments Z.of_nat: simpl never.
+Local Arguments Z.modulo : simpl never.
+Local Arguments Z.pow: simpl never.
+Local Arguments Z.sub: simpl never.
+Local Arguments Registers.reg_class.all: simpl never.
+
+Section MMIO.
+  Context {iset: InstructionSet}.
+  Context {width: Z} {BW: Bitwidth width}.
+  Context {bitwidth_iset : FlatToRiscvCommon.bitwidth_iset width iset}.
+  Context {word: Word.Interface.word width}.
+  Context {word_ok: word.ok word}.
+  Context {word_riscv_ok: word.riscv_ok word}.
+  Context {mem: map.map word byte}.
+  Context {mem_ok: map.ok mem}.
+  Context {locals: map.map Z word}.
+  Context {locals_ok: map.ok locals}.
+  Context {funname_env: forall T, map.map String.string T}.
+  Context {funname_env_ok: forall T, map.ok (funname_env T)}.
+
+  Add Ring wring : (word.ring_theory (word := word))
+      (preprocess [autorewrite with rew_word_morphism],
+       morphism (word.ring_morph (word := word)),
+       constants [word_cst]).
+
+  Definition compile_ext_call(_: funname_env Z)(_ _: Z)(s: stmt Z) :=
+      match s with
+      | SInteract resvars action argvars => compile_interact resvars action argvars
+      | _ => []
+      end.
+
+(*
+  Lemma load4bytes_in_MMIO_is_None: forall (m: mem) (addr: word),
+      map.undef_on m isMMIOAddr ->
+      isMMIOAddr addr ->
+      Memory.load_bytes 4 m addr = None.
+  Proof.
+    intros. unfold Memory.load_bytes, map.undef_on, map.agree_on, map.getmany_of_tuple in *.
+    simpl.
+    rewrite H by assumption.
+    rewrite map.get_empty.
+    reflexivity.
+  Qed.
+
+  Lemma loadWord_in_MMIO_is_None: forall (m: mem) (addr: word),
+      map.undef_on m isMMIOAddr ->
+      isMMIOAddr addr ->
+      Memory.loadWord m addr = None.
+  Proof.
+    intros. unfold Memory.loadWord.
+    apply load4bytes_in_MMIO_is_None; assumption.
+  Qed.
+
+  Lemma storeWord_in_MMIO_is_None: forall (m: mem) (addr: word) v,
+      map.undef_on m isMMIOAddr ->
+      isMMIOAddr addr ->
+      Memory.storeWord m addr v = None.
+  Proof.
+    unfold Memory.storeWord. intros. unfold Memory.store_bytes.
+    rewrite load4bytes_in_MMIO_is_None; auto.
+  Qed.
+*)
+
+  Ltac contrad := contradiction || discriminate || congruence.
+
+  (* TODO: why are these here? *)
+  Arguments LittleEndian.combine: simpl never. (* TODO can we put this next to its definition? *)
+  Arguments mcomp_sat: simpl never.
+  Arguments LittleEndian.split: simpl never.
+  Local Arguments String.eqb: simpl never.
+
+  Ltac step :=
+    match goal with
+    |- free.interp interp_action ?p ?s ?post =>
+      let p' := eval hnf in p in
+      change (free.interp interp_action p' s post);
+      rewrite free.interp_act;
+      cbn [interp_action interpret_action snd fst];
+        simpl_MetricRiscvMachine_get_set
+    | |- load ?n ?ctx ?a ?s ?k =>
+        let g' := eval cbv beta delta [load] in (load n ctx a s k) in
+        change g';
+        simpl_MetricRiscvMachine_get_set
+    | _ => progress cbn [free.bind]
+    | |- store ?n ?ctx ?a ?v ?s ?k =>
+        let g' := eval cbv beta delta [store] in (store n ctx a v s k) in
+        change g';
+        simpl_MetricRiscvMachine_get_set
+    | _ => progress cbn [free.bind]
+    | _ => rewrite free.interp_ret
+    end.
+
+  (* these are abstract and used both on the bedrock2 level and in riscv *)
+  Context {mmio_ext_calls: MemoryMappedExtCalls}.
+
+  Lemma compile_ext_call_correct: forall resvars extcall argvars,
+      FlatToRiscvCommon.compiles_FlatToRiscv_correctly compile_ext_call compile_ext_call
+        (FlatImp.SInteract resvars extcall argvars).
+  Proof.
+    unfold FlatToRiscvCommon.compiles_FlatToRiscv_correctly. simpl. intros.
+    inversion H.
+    subst resvars0 extcall argvars0 initialTrace initialMH initialRegsH
+      initialMetricsH postH. clear H.
+    destruct H5 as (? & ? & V_resvars & V_argvars).
+    fwd.
+    lazymatch goal with
+    | H: ext_spec _ _ _ _ _ |- _ => inversion H
+    end.
+  Abort.
+
+End MMIO.
